mech-uvl Dafny formalization: analyses and frontend

src/dafny/extlib/core.dfy
@@ -12,36 +12,8 @@ module ExtLib {
 
   }
 
-  module SeqFold {
+  module Algebra {
 
-    function sfold<T, U>(f: (T, U) -> U, init: U, s: seq<T>): U
-      decreases |s|
-    {
-      if |s| == 0 then
-        init
-      else
-        f(s[0], sfold(f, init, s[1..]))
-    }
-
-    lemma FoldApp<T,U>(f: (T, U) -> U, init: U, s1: seq<T>, s2: seq<T>)
-      ensures sfold(f, init, s1+s2) == sfold(f, sfold(f, init, s2), s1)
-    {
-      if |s1| == 0 {
-        assert s1+s2 == s2;
-      } else {
-        assert (s1+s2)[0] == s1[0];
-        assert (s1+s2)[1..] == s1[1..] + s2;
-        calc {
-          sfold(f, init, s1+s2);
-        == { }
-          f(s1[0], sfold(f, init, s1[1..]+s2));
-        == { FoldApp(f, init, s1[1..], s2); }
-          f(s1[0], sfold(f, sfold(f, init, s2), s1[1..]));
-        }
-      }
-    }
-
-    // Algebraic properties needed for lemmas on sfold
     ghost predicate LeftIdentity<T(!new)>(f: (T,T)-> T, neutral: T){
       forall x: T :: f(neutral, x) == x
     }
@@ -54,104 +26,122 @@ module ExtLib {
       forall x, y, z: T :: f(x, (f(y, z))) == f(f(x, y), z)
     }
 
+  }
+
+
+  /*
+    module SeqFoldRight {
+  
+      function FoldR<T, U>(f: (T, U) -> U, init: U, s: seq<T>): U
+        decreases |s|
+      {
+        if |s| == 0 then
+          init
+        else
+          f(s[0], FoldR(f, init, s[1..]))
+      }
+  
+      lemma FoldApp<T,U>(f: (T, U) -> U, init: U, s1: seq<T>, s2: seq<T>)
+        ensures FoldR(f, init, s1+s2) == FoldR(f, FoldR(f, init, s2), s1)
+      {
+        if |s1| == 0 {
+          assert s1+s2 == s2;
+        } else {
+          assert (s1+s2)[0] == s1[0];
+          assert (s1+s2)[1..] == s1[1..] + s2;
+          calc {
+            FoldR(f, init, s1+s2);
+          == { }
+            f(s1[0], FoldR(f, init, s1[1..]+s2));
+          == { FoldApp(f, init, s1[1..], s2); }
+            f(s1[0], FoldR(f, FoldR(f, init, s2), s1[1..]));
+          }
+        }
+      }
+  */
+
+  module SeqProperties {
+    import opened S = Std.Collections.Seq
+    import opened Algebra
+
     lemma FoldAppAssoc<T(!new)> (s1: seq<T>, s2: seq<T>, init: T, f: (T, T) -> T)
       requires LeftIdentity(f, init)
       requires Assoc(f)
-      ensures sfold(f, init, s1+s2) == f(sfold(f, init, s1), sfold(f, init, s2))
+      ensures FoldRight(f, s1+s2, init) == f(FoldRight(f, s1, init), FoldRight(f, s2, init))
     {
       if |s1| == 0 {
         calc {
-          sfold(f, init, s1+s2);
+          FoldRight(f, s1+s2, init);
         == { assert [] + s2 == s2; }
-          sfold(f, init, s2);
+          FoldRight(f, s2, init);
         == { }
-          f(init, sfold(f, init, s2));
+          f(init, FoldRight(f, s2, init));
         == {}
-          f(sfold(f, init, s1), sfold(f, init, s2));
+          f(FoldRight(f, s1, init), FoldRight(f, s2, init));
         }
       } else {
         FoldAppAssoc(s1[1..], s2, init, f);
         assert (s1+s2)[0] == s1[0];
         assert (s1+s2)[1..] == s1[1..]+s2;
         calc {
-          sfold(f, init, s1+s2);
+          FoldRight(f, s1+s2, init);
         == {}
-          f(s1[0], sfold(f, init, s1[1..]+s2));
+          f(s1[0], FoldRight(f, s1[1..]+s2, init));
         == {}
-          f(s1[0], f(sfold(f, init, s1[1..]), sfold(f, init, s2)));
+          f(s1[0], f(FoldRight(f, s1[1..], init), FoldRight(f, s2, init)));
         == {}
-          f(sfold(f, init, s1), sfold(f, init, s2));
+          f(FoldRight(f, s1, init), FoldRight(f, s2, init));
         }
       }
     }
+
   }
 
-  module SeqFoldLeft {
 
-    function sfoldl<T, U>(f: (U, T) -> U, init: U, s: seq<T>): U
-      decreases |s|
-    {
-      if |s| == 0 then
-        init
-      else
-        sfoldl(f, f(init, s[0]), s[1..])
-    }
-
-    lemma FoldApp<T,U>(f: (U, T) -> U, init: U, s1: seq<T>, s2: seq<T>)
-      ensures sfoldl(f, init, s1+s2) == sfoldl(f, sfoldl(f, init, s1), s2)
-    {
-      if |s1| == 0 {
-        assert s1+s2 == s2;
-      } else {
-        assert (s1+s2)[0] == s1[0];
-        assert (s1+s2)[1..] == s1[1..] + s2;
-        FoldApp(f, f(init, s1[0]), s1[1..], s2);
-      }
-    }
-  }
 
   module SeqMap {
-    import opened SeqFoldLeft
+    import opened Std.Collections.Seq
+    import opened SeqProperties
 
-    function smap<A,B>(f: A->B, s: seq<A>): seq<B>{
+    function FMap<A,B>(f: A->B, s: seq<A>): seq<B>{
       if |s| == 0
       then []
-      else [f(s[0])] + smap(f, s[1..])
+      else [f(s[0])] + FMap(f, s[1..])
     }
 
-    lemma MapApp<A,B>(f: A->B, s1: seq<A>, s2:seq<A>)
-      ensures smap(f, s1+s2) == smap(f, s1) + smap(f, s2)
+    lemma FMapApp<A,B>(f: A->B, s1: seq<A>, s2:seq<A>)
+      ensures FMap(f, s1+s2) == FMap(f, s1) + FMap(f, s2)
     {
       if |s1| == 0 {
         assert s1+s2 == s2;
       } else {
         assert (s1+s2)[0] == s1[0];
         assert (s1+s2)[1..] == s1[1..]+s2;
-        MapApp(f, s1[1..], s2);
+        FMapApp(f, s1[1..], s2);
       }
     }
 
-    lemma MapExt<A,B>(s: seq<A>, f1: A->B, f2: A->B)
+    lemma FMapExt<A,B>(s: seq<A>, f1: A->B, f2: A->B)
       requires forall x :: x in s ==> f1(x) == f2(x)
-      ensures smap(f1, s) == smap(f2, s)
+      ensures FMap(f1, s) == FMap(f2, s)
     {
       if |s| == 0 {
       } else {
-        MapExt(s[1..], f1, f2);
+        FMapExt(s[1..], f1, f2);
       }
     }
 
-    lemma MapMap<A,B,C>(f: A->B, g: B->C, s: seq<A>)
-      ensures smap(g, smap(f, s)) == smap((x: A) => g(f(x)), s)
+    lemma FMapFMap<A,B,C>(f: A->B, g: B->C, s: seq<A>)
+      ensures FMap(g, FMap(f, s)) == FMap((x: A) => g(f(x)), s)
     {
       if |s| == 0 {
       } else {
-        MapMap(f, g, s[1..]);
+        FMapFMap(f, g, s[1..]);
       }
     }
 
     lemma FoldMapLeft<A,B,C>(f: (A, B)->A, g:C->B, s: seq<C>, init: A)
-      ensures sfoldl(f, init, smap(g, s)) == sfoldl((a, c) => f(a, g(c)), init, s)
+      ensures FoldLeft(f, init, FMap(g, s)) == FoldLeft((a, c) => f(a, g(c)), init, s)
     {
       if |s| == 0 {
       } else {
@@ -161,33 +151,15 @@ module ExtLib {
 
   }
 
-  module ForAll {
-    import opened SeqFold
-
-    // A computable forall on sequences
-    function ForAll<T>(p: T->bool, s: seq<T>) : bool
-    {
-      sfold((e, t)=> p(e) && t, true, s)
-    }
-
-    lemma ForAll_forall<T>(s: seq<T>, p: T->bool)
-      ensures (forall i :: 0 <= i < |s| ==>p(s[i])) <==> ForAll(p, s)
-    {
-      if |s| == 0 {
-      } else {
-        ForAll_forall(s[1..], p);
-      }
-    }
-  }
-
   module Sum {
 
     module EInt {
-      import opened SeqFold
+      import opened Std.Collections.Seq
+      import opened Algebra
 
       // Sum on integers
       function sum(numbers: seq<int>): int {
-        sfold((x,y)=>(x+y), 0, numbers)
+        FoldRight((x,y)=>(x+y), numbers, 0)
       }
 
       lemma sumHd(xs: seq<int>)
@@ -205,11 +177,12 @@ module ExtLib {
     }
 
     module Float {
-      import opened SeqFold
+      import opened Std.Collections.Seq
+      import opened Algebra
 
       // Sum on real numbers
       function sum(numbers: seq<real>): real {
-        sfold((x,y)=>(x+y), 0., numbers)
+        FoldRight((x,y)=>(x+y), numbers, 0.)
       }
 
       lemma sumHd(xs: seq<real>)
@@ -228,11 +201,12 @@ module ExtLib {
     }
 
     module Nat {
-      import opened SeqFold
+      import opened Std.Collections.Seq
+      import opened Algebra
 
       // Sum on natural numbers
       function sum(numbers: seq<nat>): nat {
-        sfold((x,y)=>(x+y), 0, numbers)
+        FoldRight((x,y)=>(x+y), numbers, 0)
       }
 
       lemma sumHd(xs: seq<nat>)
@@ -248,6 +222,7 @@ module ExtLib {
         ensures Assoc<nat>((x,y)=>(x+y))
       {}
     }
+
   }
 
   module SeqNoDup {
@@ -263,37 +238,38 @@ module ExtLib {
 
   module SetToSeq {
 
-    ghost function set2seq<T(!new)>(s: set<T>): seq<T>
-      ensures forall x :: x in s <==> x in set2seq(s)
-      ensures |set2seq(s)| == |s|
+    ghost function Set2Seq<T(!new)>(s: set<T>): seq<T>
+      ensures forall x :: x in s <==> x in Set2Seq(s)
+      ensures |Set2Seq(s)| == |s|
       decreases |s|
     {
       if s == {} then
         []
       else
         var x :| x in s;
-        [x] + set2seq(s - {x})
+        [x] + Set2Seq(s - {x})
     }
 
   }
 
   module SeqMapMerge {
-    import opened SeqFold
+    import opened Std.Collections.Seq
 
     function Merge<A,B>(chunks: seq<map<A, B>>): map<A, B>
     {
-      sfold((chunk, acc) => chunk + acc, map[], chunks)
+      FoldRight((chunk, acc) => chunk + acc, chunks, map[])
     }
 
   }
 
   module SeqSetUnion {
-    import opened SeqFoldLeft
+    import opened Std.Collections.Seq
 
     function Union<A>(sets: seq<set<A>>): set<A>
     {
-      sfoldl((s1,s2)=>s1+s2, {}, sets)
+      FoldRight((s1,s2)=>s1+s2, sets, {})
     }
+
   }
 
 }
