src/dafny/frontend/external.dfy
@@ -1,0 +1,23 @@
+// Copyright (C) 2026 Université d'Orléans
+// Author: Frédéric Loulergue
+// SPDX-License-Identifier: GPL-3.0-only
+
+// This module declares the trusted parser entry point for UVL source files.
+
+module UVL_Parse {
+  import opened ExtLib.Option
+  import opened UVL_Syntax
+
+  // Parses one UVL file in the import space rooted at rootPath. The second
+  // argument is the root-relative UVL path of the model to parse, where None
+  // denotes the root model itself. The ghost set makes explicit the fact that
+  // there is only a finite set of files that can be possibly imported from the
+  // root, because the number of files in a filesystem is finite.
+  method {:extern "UvlExternal", "Parse"} {:axiom} Parse(
+    rootPath: string,
+    path: option<Reference>,
+    ghost accessiblePaths: set<option<Reference>>
+  ) returns (model: option<FeatureModel>)
+    ensures path !in accessiblePaths ==> model.None?
+    ensures model.Some? ==> path in accessiblePaths
+}
